added shell

Sodium.lean
@@ -1,3 +1,25 @@
-import «Sodium».Crypto.Monad
-import «Sodium».Data.Digest
-import «Sodium».Lean.Syntax
+import «Sodium».Typo.Frontend.Qwerty
+
+universe «u»
+
+open Lean Sodium Crypto Ethos
+
+/--
+HACK: This is a workaround for ensuring that `aesop`'s proof reconstruction works.
+-/
+@[aesop norm unfold (rule_sets := [«external»])]
+instance prompt : Inhabited Prop := Universal.prompt.{0}
+
+@[aesop norm forward (rule_sets := [«external»])]
+def construct : @default Prop prompt := by
+  unfold prompt Universal.prompt
+  simp only [Encodable.encodek, implies_true, and_self]
+
+@[aesop unsafe 0% apply (rule_sets := [«external»])] -- 0% to force termination before any "impossible" tactics are run.
+def destruct (fwd : Universal.Forward.{«u»}) : Universal Universal.Destruct.{«u»} := by
+  refine ⟨default, fun α => ?_⟩
+  have : Observable := α construct
+  exact ⟨fwd this.carrier⟩
+
+example : Universal Universal.Destruct.{0} := by
+  aesop? (rule_sets := [«standard», «cautious», «external»])
