Sodium/Shell/Basic.lean
@@ -1,0 +1,8 @@
+import Sodium.Typography.Frontend.Qwerty
+
+open Lean Sodium Ethos
+
+set_option trace.aesop true
+
+example : Universal (PLift (∀ α, (Observable.Shape.push α).pull = α)) := by
+  aesop? (rule_sets := [«standard», «cautious», «external»]) (config := {warnOnNonterminal := false})
