Sodium/Typo/Latin.lean
@@ -1,0 +1,241 @@
+import Sodium.Typo.Emulator
+
+open Lean Elab Tactic
+
+variable {σ}
+
+namespace Typo
+
+protected def Latin.Shape : PFunctor where
+  A := Shape
+  B | shape% 'a' | shape% 'A'
+    | shape% 'b' | shape% 'B'
+    | shape% 'c' | shape% 'C'
+    | shape% 'd' | shape% 'D'
+    | shape% 'e' | shape% 'E'
+    | shape% 'f' | shape% 'F'
+    | shape% 'g' | shape% 'G'
+    | shape% 'h' | shape% 'H'
+    | shape% 'i' | shape% 'I'
+    | shape% 'j' | shape% 'J'
+    | shape% 'k' | shape% 'K'
+    | shape% 'l' | shape% 'L'
+    | shape% 'm' | shape% 'M'
+    | shape% 'n' | shape% 'N'
+    | shape% 'o' | shape% 'O'
+    | shape% 'p' | shape% 'P'
+    | shape% 'q' | shape% 'Q'
+    | shape% 'r' | shape% 'R'
+    | shape% 's' | shape% 'S'
+    | shape% 't' | shape% 'T'
+    | shape% 'u' | shape% 'U'
+    | shape% 'v' | shape% 'V'
+    | shape% 'w' | shape% 'W'
+    | shape% 'x' | shape% 'X'
+    | shape% 'y' | shape% 'Y'
+    | shape% 'z' | shape% 'Z' => PUnit
+    | _ => PEmpty
+
+abbrev Latin (σ) := Emulator σ ⊚ Latin.Shape.{0}
+
+@[simp] theorem latin_idx : Latin.Shape.A = Shape := rfl
+
+@[simp] theorem latin_idx_alpha : Latin.Shape.B (shape% 'a') = PUnit := rfl
+@[simp] theorem latin_idx_beta : Latin.Shape.B (shape% 'b') = PUnit := rfl
+@[simp] theorem latin_idx_gamma : Latin.Shape.B (shape% 'c') = PUnit := rfl
+@[simp] theorem latin_idx_delta : Latin.Shape.B (shape% 'd') = PUnit := rfl
+@[simp] theorem latin_idx_epsilon : Latin.Shape.B (shape% 'e') = PUnit := rfl
+@[simp] theorem latin_idx_zeta : Latin.Shape.B (shape% 'f') = PUnit := rfl
+@[simp] theorem latin_idx_eta : Latin.Shape.B (shape% 'g') = PUnit := rfl
+@[simp] theorem latin_idx_theta : Latin.Shape.B (shape% 'h') = PUnit := rfl
+@[simp] theorem latin_idx_iota : Latin.Shape.B (shape% 'i') = PUnit := rfl
+@[simp] theorem latin_idx_kappa : Latin.Shape.B (shape% 'j') = PUnit := rfl
+@[simp] theorem latin_idx_lambda : Latin.Shape.B (shape% 'k') = PUnit := rfl
+@[simp] theorem latin_idx_mu : Latin.Shape.B (shape% 'l') = PUnit := rfl
+@[simp] theorem latin_idx_nu : Latin.Shape.B (shape% 'm') = PUnit := rfl
+@[simp] theorem latin_idx_xi : Latin.Shape.B (shape% 'n') = PUnit := rfl
+@[simp] theorem latin_idx_omicron : Latin.Shape.B (shape% 'o') = PUnit := rfl
+@[simp] theorem latin_idx_pi : Latin.Shape.B (shape% 'p') = PUnit := rfl
+@[simp] theorem latin_idx_rho : Latin.Shape.B (shape% 'q') = PUnit := rfl
+@[simp] theorem latin_idx_sigma : Latin.Shape.B (shape% 'r') = PUnit := rfl
+@[simp] theorem latin_idx_tau : Latin.Shape.B (shape% 's') = PUnit := rfl
+@[simp] theorem latin_idx_upsilon : Latin.Shape.B (shape% 't') = PUnit := rfl
+@[simp] theorem latin_idx_phi : Latin.Shape.B (shape% 'u') = PUnit := rfl
+@[simp] theorem latin_idx_chi : Latin.Shape.B (shape% 'v') = PUnit := rfl
+@[simp] theorem latin_idx_psi : Latin.Shape.B (shape% 'w') = PUnit := rfl
+@[simp] theorem latin_idx_omega : Latin.Shape.B (shape% 'x') = PUnit := rfl
+@[simp] theorem latin_idx_why : Latin.Shape.B (shape% 'y') = PUnit := rfl
+@[simp] theorem latin_idx_zed : Latin.Shape.B (shape% 'z') = PUnit := rfl
+
+@[simp] theorem latin_idx_Alpha : Latin.Shape.B (shape% 'A') = PUnit := rfl
+@[simp] theorem latin_idx_Beta : Latin.Shape.B (shape% 'B') = PUnit := rfl
+@[simp] theorem latin_idx_Gamma : Latin.Shape.B (shape% 'C') = PUnit := rfl
+@[simp] theorem latin_idx_Delta : Latin.Shape.B (shape% 'D') = PUnit := rfl
+@[simp] theorem latin_idx_Epsilon : Latin.Shape.B (shape% 'E') = PUnit := rfl
+@[simp] theorem latin_idx_Zeta : Latin.Shape.B (shape% 'F') = PUnit := rfl
+@[simp] theorem latin_idx_Eta : Latin.Shape.B (shape% 'G') = PUnit := rfl
+@[simp] theorem latin_idx_Theta : Latin.Shape.B (shape% 'H') = PUnit := rfl
+@[simp] theorem latin_idx_Iota : Latin.Shape.B (shape% 'I') = PUnit := rfl
+@[simp] theorem latin_idx_Kappa : Latin.Shape.B (shape% 'J') = PUnit := rfl
+@[simp] theorem latin_idx_Lambda : Latin.Shape.B (shape% 'K') = PUnit := rfl
+@[simp] theorem latin_idx_Mu : Latin.Shape.B (shape% 'L') = PUnit := rfl
+@[simp] theorem latin_idx_Nu : Latin.Shape.B (shape% 'M') = PUnit := rfl
+@[simp] theorem latin_idx_Xi : Latin.Shape.B (shape% 'N') = PUnit := rfl
+@[simp] theorem latin_idx_Omicron : Latin.Shape.B (shape% 'O') = PUnit := rfl
+@[simp] theorem latin_idx_Pi : Latin.Shape.B (shape% 'P') = PUnit := rfl
+@[simp] theorem latin_idx_Rho : Latin.Shape.B (shape% 'Q') = PUnit := rfl
+@[simp] theorem latin_idx_Sigma : Latin.Shape.B (shape% 'R') = PUnit := rfl
+@[simp] theorem latin_idx_Tau : Latin.Shape.B (shape% 'S') = PUnit := rfl
+@[simp] theorem latin_idx_Upsilon : Latin.Shape.B (shape% 'T') = PUnit := rfl
+@[simp] theorem latin_idx_Phi : Latin.Shape.B (shape% 'U') = PUnit := rfl
+@[simp] theorem latin_idx_Chi : Latin.Shape.B (shape% 'V') = PUnit := rfl
+@[simp] theorem latin_idx_Psi : Latin.Shape.B (shape% 'W') = PUnit := rfl
+@[simp] theorem latin_idx_Omega : Latin.Shape.B (shape% 'X') = PUnit := rfl
+@[simp] theorem latin_idx_Why : Latin.Shape.B (shape% 'Y') = PUnit := rfl
+@[simp] theorem latin_idx_Zed : Latin.Shape.B (shape% 'Z') = PUnit := rfl
+
+@[simp] theorem latin_idx_none : Latin.Shape.B (default : Shape) = PEmpty := rfl
+
+namespace Latin.Syntax
+
+private def mkExactULiftChar (c : Char) : Syntax.Tactic :=
+  ⟨Syntax.node .none ``Lean.Parser.Tactic.exact #[
+    Syntax.atom .none "exact",
+    Syntax.node .none ``Lean.Parser.Term.anonymousCtor #[
+      Syntax.atom .none "⟨",
+      Syntax.mkCharLit c,
+      Syntax.atom .none "⟩"
+    ]
+  ]⟩
+
+protected def a : Syntax.Tactic := mkExactULiftChar 'a'
+protected def b : Syntax.Tactic := mkExactULiftChar 'b'
+protected def c : Syntax.Tactic := mkExactULiftChar 'c'
+protected def d : Syntax.Tactic := mkExactULiftChar 'd'
+protected def e : Syntax.Tactic := mkExactULiftChar 'e'
+protected def f : Syntax.Tactic := mkExactULiftChar 'f'
+protected def g : Syntax.Tactic := mkExactULiftChar 'g'
+protected def h : Syntax.Tactic := mkExactULiftChar 'h'
+protected def i : Syntax.Tactic := mkExactULiftChar 'i'
+protected def j : Syntax.Tactic := mkExactULiftChar 'j'
+protected def k : Syntax.Tactic := mkExactULiftChar 'k'
+protected def l : Syntax.Tactic := mkExactULiftChar 'l'
+protected def m : Syntax.Tactic := mkExactULiftChar 'm'
+protected def n : Syntax.Tactic := mkExactULiftChar 'n'
+protected def o : Syntax.Tactic := mkExactULiftChar 'o'
+protected def p : Syntax.Tactic := mkExactULiftChar 'p'
+protected def q : Syntax.Tactic := mkExactULiftChar 'q'
+protected def r : Syntax.Tactic := mkExactULiftChar 'r'
+protected def s : Syntax.Tactic := mkExactULiftChar 's'
+protected def t : Syntax.Tactic := mkExactULiftChar 't'
+protected def u : Syntax.Tactic := mkExactULiftChar 'u'
+protected def v : Syntax.Tactic := mkExactULiftChar 'v'
+protected def w : Syntax.Tactic := mkExactULiftChar 'w'
+protected def x : Syntax.Tactic := mkExactULiftChar 'x'
+protected def y : Syntax.Tactic := mkExactULiftChar 'y'
+protected def z : Syntax.Tactic := mkExactULiftChar 'z'
+
+protected def A : Syntax.Tactic := mkExactULiftChar 'A'
+protected def B : Syntax.Tactic := mkExactULiftChar 'B'
+protected def C : Syntax.Tactic := mkExactULiftChar 'C'
+protected def D : Syntax.Tactic := mkExactULiftChar 'D'
+protected def E : Syntax.Tactic := mkExactULiftChar 'E'
+protected def F : Syntax.Tactic := mkExactULiftChar 'F'
+protected def G : Syntax.Tactic := mkExactULiftChar 'G'
+protected def H : Syntax.Tactic := mkExactULiftChar 'H'
+protected def I : Syntax.Tactic := mkExactULiftChar 'I'
+protected def J : Syntax.Tactic := mkExactULiftChar 'J'
+protected def K : Syntax.Tactic := mkExactULiftChar 'K'
+protected def L : Syntax.Tactic := mkExactULiftChar 'L'
+protected def M : Syntax.Tactic := mkExactULiftChar 'M'
+protected def N : Syntax.Tactic := mkExactULiftChar 'N'
+protected def O : Syntax.Tactic := mkExactULiftChar 'O'
+protected def P : Syntax.Tactic := mkExactULiftChar 'P'
+protected def Q : Syntax.Tactic := mkExactULiftChar 'Q'
+protected def R : Syntax.Tactic := mkExactULiftChar 'R'
+protected def S : Syntax.Tactic := mkExactULiftChar 'S'
+protected def T : Syntax.Tactic := mkExactULiftChar 'T'
+protected def U : Syntax.Tactic := mkExactULiftChar 'U'
+protected def V : Syntax.Tactic := mkExactULiftChar 'V'
+protected def W : Syntax.Tactic := mkExactULiftChar 'W'
+protected def X : Syntax.Tactic := mkExactULiftChar 'X'
+protected def Y : Syntax.Tactic := mkExactULiftChar 'Y'
+protected def Z : Syntax.Tactic := mkExactULiftChar 'Z'
+
+end Syntax
+
+syntax "latin% " term ", " char ", " term : term
+
+elab "latin% " τ:term ", " γ:char ", " stx:term : tactic => do
+  let x := mkIdent `«x»
+  evalTactic <| ← `(tactic|refine ⟨⟨commit% $τ, $γ, $stx, fun _ => shape% $γ⟩, fun $x => ?_⟩)
+  evalTactic <| ← `(tactic|obtain ⟨$x, _⟩ := $x)
+  evalTactic <| ← `(tactic|exact $x)
+
+variable {τ : Sodium σ}
+
+protected def a : (Latin σ) (TermElabM Shape) := by latin% τ, 'a', Syntax.a
+protected def b : (Latin σ) (TermElabM Shape) := by latin% τ, 'b', Syntax.b
+protected def c : (Latin σ) (TermElabM Shape) := by latin% τ, 'c', Syntax.c
+protected def d : (Latin σ) (TermElabM Shape) := by latin% τ, 'd', Syntax.d
+protected def e : (Latin σ) (TermElabM Shape) := by latin% τ, 'e', Syntax.e
+protected def f : (Latin σ) (TermElabM Shape) := by latin% τ, 'f', Syntax.f
+protected def g : (Latin σ) (TermElabM Shape) := by latin% τ, 'g', Syntax.g
+protected def h : (Latin σ) (TermElabM Shape) := by latin% τ, 'h', Syntax.h
+protected def i : (Latin σ) (TermElabM Shape) := by latin% τ, 'i', Syntax.i
+protected def j : (Latin σ) (TermElabM Shape) := by latin% τ, 'j', Syntax.j
+protected def k : (Latin σ) (TermElabM Shape) := by latin% τ, 'k', Syntax.k
+protected def l : (Latin σ) (TermElabM Shape) := by latin% τ, 'l', Syntax.l
+protected def m : (Latin σ) (TermElabM Shape) := by latin% τ, 'm', Syntax.m
+protected def n : (Latin σ) (TermElabM Shape) := by latin% τ, 'n', Syntax.n
+protected def o : (Latin σ) (TermElabM Shape) := by latin% τ, 'o', Syntax.o
+protected def p : (Latin σ) (TermElabM Shape) := by latin% τ, 'p', Syntax.p
+protected def q : (Latin σ) (TermElabM Shape) := by latin% τ, 'q', Syntax.q
+protected def r : (Latin σ) (TermElabM Shape) := by latin% τ, 'r', Syntax.r
+protected def s : (Latin σ) (TermElabM Shape) := by latin% τ, 's', Syntax.s
+protected def t : (Latin σ) (TermElabM Shape) := by latin% τ, 't', Syntax.t
+protected def u : (Latin σ) (TermElabM Shape) := by latin% τ, 'u', Syntax.u
+protected def v : (Latin σ) (TermElabM Shape) := by latin% τ, 'v', Syntax.v
+protected def w : (Latin σ) (TermElabM Shape) := by latin% τ, 'w', Syntax.w
+protected def x : (Latin σ) (TermElabM Shape) := by latin% τ, 'x', Syntax.x
+protected def y : (Latin σ) (TermElabM Shape) := by latin% τ, 'y', Syntax.y
+protected def z : (Latin σ) (TermElabM Shape) := by latin% τ, 'z', Syntax.z
+
+protected def A : (Latin σ) (TermElabM Shape) := by latin% τ, 'A', Syntax.A
+protected def B : (Latin σ) (TermElabM Shape) := by latin% τ, 'B', Syntax.B
+protected def C : (Latin σ) (TermElabM Shape) := by latin% τ, 'C', Syntax.C
+protected def D : (Latin σ) (TermElabM Shape) := by latin% τ, 'D', Syntax.D
+protected def E : (Latin σ) (TermElabM Shape) := by latin% τ, 'E', Syntax.E
+protected def F : (Latin σ) (TermElabM Shape) := by latin% τ, 'F', Syntax.F
+protected def G : (Latin σ) (TermElabM Shape) := by latin% τ, 'G', Syntax.G
+protected def H : (Latin σ) (TermElabM Shape) := by latin% τ, 'H', Syntax.H
+protected def I : (Latin σ) (TermElabM Shape) := by latin% τ, 'I', Syntax.I
+protected def J : (Latin σ) (TermElabM Shape) := by latin% τ, 'J', Syntax.J
+protected def K : (Latin σ) (TermElabM Shape) := by latin% τ, 'K', Syntax.K
+protected def L : (Latin σ) (TermElabM Shape) := by latin% τ, 'L', Syntax.L
+protected def M : (Latin σ) (TermElabM Shape) := by latin% τ, 'M', Syntax.M
+protected def N : (Latin σ) (TermElabM Shape) := by latin% τ, 'N', Syntax.N
+protected def O : (Latin σ) (TermElabM Shape) := by latin% τ, 'O', Syntax.O
+protected def P : (Latin σ) (TermElabM Shape) := by latin% τ, 'P', Syntax.P
+protected def Q : (Latin σ) (TermElabM Shape) := by latin% τ, 'Q', Syntax.Q
+protected def R : (Latin σ) (TermElabM Shape) := by latin% τ, 'R', Syntax.R
+protected def S : (Latin σ) (TermElabM Shape) := by latin% τ, 'S', Syntax.S
+protected def T : (Latin σ) (TermElabM Shape) := by latin% τ, 'T', Syntax.T
+protected def U : (Latin σ) (TermElabM Shape) := by latin% τ, 'U', Syntax.U
+protected def V : (Latin σ) (TermElabM Shape) := by latin% τ, 'V', Syntax.V
+protected def W : (Latin σ) (TermElabM Shape) := by latin% τ, 'W', Syntax.W
+protected def X : (Latin σ) (TermElabM Shape) := by latin% τ, 'X', Syntax.X
+protected def Y : (Latin σ) (TermElabM Shape) := by latin% τ, 'Y', Syntax.Y
+protected def Z : (Latin σ) (TermElabM Shape) := by latin% τ, 'Z', Syntax.Z
+
+@[aesop norm unfold (rule_sets := [«standard»])]
+protected def map {α β} := @PFunctor.map α β (Latin σ)
+
+open Sodium Crypto Ethos in
+def quantize (γ : (Latin σ) (TermElabM Shape)) (scope : ScopeName) : (Latin σ) (CryptoM τ Observable) := by
+  refine Latin.map (fun γ => ?_) γ
+  exact do let γ ← Aesop.runTermElabMAsCoreM γ; γ.quantize scope
+
+end Latin
+
+end Typo
